verified/pagedb.s.dfy
@@ -23,7 +23,7 @@ datatype PageDbEntryTyped
 
 datatype L2PTE
     = SecureMapping(page: PageNr, write: bool, exec: bool)
-    | InsecureMapping(insecurePage: InsecurePageNr)
+    | InsecureMapping(insecurePage: InsecurePageNr, insecureWrite: bool)
     | NoMapping
 
 datatype PageDbEntry
@@ -37,36 +37,31 @@ predicate wellFormedPageDb(d: PageDb)
     forall n {:trigger validPageNr(n)} :: validPageNr(n) <==> n in d
 }
 
-predicate {:opaque} validPageDb(d: PageDb)
-{
-    wellFormedPageDb(d)
-    && pageDbEntriesValidRefs(d)
-    && pageDbEntriesValid(d)
-}
-
-// this is a weak predicate that simply says the page number refs are valid
+// this is a weak predicate that simply says internal refs are all in bounds
 predicate {:opaque} pageDbClosedRefs(d: PageDb)
+    ensures pageDbClosedRefs(d) ==> wellFormedPageDb(d)
 {
-    wellFormedPageDb(d) && (forall n {:trigger validPageNr(n)} :: (validPageNr(n) && d[n].PageDbEntryTyped?)
-        ==> (validPageNr(d[n].addrspace) && closedRefsPageDbEntry(d[n].entry)))
+    wellFormedPageDb(d) && forall n :: validPageNr(n) ==> closedRefsPageDbEntry(d[n])
 }
 
-lemma validPageDbImpliesClosedRefs(d: PageDb)
-    requires validPageDb(d)
-    ensures pageDbClosedRefs(d)
-    {reveal_validPageDb(); reveal_pageDbClosedRefs();}
+predicate {:opaque} validPageDb(d: PageDb)
+    ensures validPageDb(d) ==> pageDbClosedRefs(d)
+{
+    wellFormedPageDb(d) && pageDbEntriesValid(d) && pageDbEntriesValidRefs(d)
+}
 
 predicate pageDbEntriesValid(d:PageDb)
     requires wellFormedPageDb(d)
+    ensures pageDbEntriesValid(d) ==> pageDbClosedRefs(d)
 {
+    reveal_pageDbClosedRefs();
     forall n :: validPageNr(n) ==> validPageDbEntry(d, n)
 }
 
 predicate pageDbEntriesValidRefs(d: PageDb)
     requires wellFormedPageDb(d)
 {
-    forall n :: validPageNr(n) && d[n].PageDbEntryTyped? ==> 
-        pageDbEntryValidRefs(d, n)
+    forall n :: validPageNr(n) && d[n].PageDbEntryTyped? ==>  pageDbEntryValidRefs(d, n)
 }
 
 // Free pages and non-addrspace entries should have a refcount of 0
@@ -75,12 +70,12 @@ predicate pageDbEntryValidRefs(d: PageDb, n: PageNr)
 {
     var e := d[n];
     (e.PageDbEntryTyped? && e.entry.Addrspace?) ||
-        forall m : PageNr :: validPageNr(m) ==>
-            |addrspaceRefs(d, n)| == 0
+        |addrspaceRefs(d, n)| == 0
 }
 
 predicate validPageDbEntry(d: PageDb, n: PageNr)
     requires wellFormedPageDb(d) && validPageNr(n)
+    //ensures validPageDbEntry(d, n) ==> closedRefsPageDbEntry(d[n])
 {
     var e := d[n];
     e.PageDbEntryFree? ||
@@ -91,63 +86,48 @@ predicate validPageDbEntryTyped(d: PageDb, n: PageNr)
     requires wellFormedPageDb(d) && validPageNr(n)
     requires d[n].PageDbEntryTyped?
 {
-    var e := d[n].entry;
-    closedRefsPageDbEntry(e) && pageDbEntryOk(d, n)
-}
-
-predicate isAddrspace(d: PageDb, n: PageNr)
-{
-    wellFormedPageDb(d) && validPageNr(n) && d[n].PageDbEntryTyped? && d[n].entry.Addrspace?
-}
-
-// The addrspace of the thing pointed to by n is stopped
-predicate stoppedAddrspace(d: PageDb, n: PageNr)
-    requires wellFormedPageDb(d) && validPageNr(n)
-    requires d[n].PageDbEntryTyped?
-{
-    var a := d[n].addrspace;
-    isAddrspace(d, a) && d[a].entry.state == StoppedState
-}
-
-predicate pageDbEntryOk(d: PageDb, n: PageNr)
-    requires wellFormedPageDb(d) && validPageNr(n)
-    requires d[n].PageDbEntryTyped?
-{
-    var entry := d[n].entry;
-    var addrspace := d[n].addrspace;
-    isAddrspace(d, addrspace)
+    closedRefsPageDbEntry(d[n]) && isAddrspace(d, d[n].addrspace)
     // Type-specific requirements
-    && ( (entry.Addrspace? && validAddrspace(d, n))
+    && (var entry := d[n].entry;
+         (entry.Addrspace? && validAddrspace(d, n))
        || (entry.L1PTable? && validL1PTable(d, n))
        || (entry.L2PTable? && validL2PTable(d, n))
        || (entry.Dispatcher?)
        || (entry.DataPage?) )
-    
+}
+
+predicate isAddrspace(d: PageDb, n: PageNr)
+{
+    wellFormedPageDb(d) && validPageNr(n)
+        && d[n].PageDbEntryTyped?
+        && d[n].entry.Addrspace?
+}
+
+predicate stoppedAddrspace(e: PageDbEntry)
+{
+    e.PageDbEntryTyped? && e.entry.Addrspace? && e.entry.state == StoppedState
 }
 
 predicate validAddrspace(d: PageDb, n: PageNr)
     requires isAddrspace(d, n)
+    requires closedRefsPageDbEntry(d[n])
 {
-        var addrspace := d[n].entry;
-        n == d[n].addrspace
+    var addrspace := d[n].entry;
+    n == d[n].addrspace
         && addrspaceL1Unique(d, n)
         && addrspace.refcount == |addrspaceRefs(d, n)|
-        && (stoppedAddrspace(d, n) ||  (
-            d[addrspace.l1ptnr].PageDbEntryTyped? &&
-            d[addrspace.l1ptnr].entry.L1PTable? &&
-            d[addrspace.l1ptnr].addrspace == n
+        && (stoppedAddrspace(d[n]) || (
+            var l1pt := d[addrspace.l1ptnr];
+            l1pt.PageDbEntryTyped? && l1pt.entry.L1PTable? && l1pt.addrspace == n
         ))
 }
 
 predicate addrspaceL1Unique(d: PageDb, n: PageNr)
-    requires wellFormedPageDb(d) && validPageNr(n)
-    requires d[n].PageDbEntryTyped? && d[n].entry.Addrspace?
+    requires isAddrspace(d, n)
 {
     var a := d[n].entry;
-    a.l1ptnr in d &&
-    forall p :: validPageNr(p) && p != a.l1ptnr &&
-        d[p].PageDbEntryTyped? && d[p].addrspace == n ==>
-        !d[p].entry.L1PTable?
+    forall p :: validPageNr(p) && p != a.l1ptnr && d[p].PageDbEntryTyped? && d[p].addrspace == n
+        ==> !d[p].entry.L1PTable?
 }
 
 // taken from ironclad set libraries
@@ -179,17 +159,16 @@ function addrspaceRefs(d: PageDb, addrspacePageNr: PageNr): set<PageNr>
 
 predicate validL1PTable(d: PageDb, n: PageNr)
     requires wellFormedPageDb(d) && validPageNr(n)
+    requires closedRefsPageDbEntry(d[n])
     requires d[n].PageDbEntryTyped? && d[n].entry.L1PTable?
-    requires var a:= d[n].addrspace; isAddrspace(d, a)
 {
-    var e := d[n];
-    var l1pt := e.entry.l1pt;
+    var l1pt := d[n].entry.l1pt;
     var a := d[n].addrspace;
-    stoppedAddrspace(d, n) || (
-        forall pte :: pte in l1pt && pte.Just? ==> ( var pteE := fromJust(pte);
-            pteE in d && d[pteE].PageDbEntryTyped? && d[pteE].addrspace == a )
+    stoppedAddrspace(d[a]) || (
         // each non-zero entry is a valid L2PT belonging to this address space
-        && forall pte :: pte in l1pt && pte.Just? ==> validL1PTE(d, fromJust(pte))
+        forall pte :: pte in l1pt && pte.Just? ==> (
+            var pteE := fromJust(pte);
+            d[pteE].PageDbEntryTyped? && d[pteE].addrspace == a && validL1PTE(d, pteE))
         // no L2PT is referenced twice
         && forall i, j :: 0 <= i < |l1pt| && 0 <= j < |l1pt| && l1pt[i].Just? && i != j
             ==> l1pt[i] != l1pt[j]
@@ -206,20 +185,16 @@ predicate validL1PTE(d: PageDb, pte: PageNr)
 
 predicate validL2PTable(d: PageDb, n: PageNr)
     requires wellFormedPageDb(d) && validPageNr(n)
+    requires closedRefsPageDbEntry(d[n])
     requires d[n].PageDbEntryTyped? && d[n].entry.L2PTable?
-    requires var a:= d[n].addrspace; isAddrspace(d, a)
 {
-    var e := d[n];
-    var l2pt := e.entry.l2pt;
-    var a:= d[n].addrspace;
-    stoppedAddrspace(d, n) || (
-        forall pte :: pte in l2pt && pte.SecureMapping? ==> (
-            var ptePg := pte.page;
-            ptePg in d && d[ptePg].PageDbEntryTyped? && d[ptePg].addrspace == a)
+    var a := d[n].addrspace;
+    stoppedAddrspace(d[a]) || (
+        forall pte :: pte in d[n].entry.l2pt && pte.SecureMapping? ==> (
         // Not needed when addrspace is stopped 
         // each secure entry is a valid data page belonging to this address space
-        && forall pte :: pte in l2pt && pte.SecureMapping?
-            ==> validL2PTE(d, pte.page)
+            var pg := pte.page;
+            d[pg].PageDbEntryTyped? && d[pg].addrspace == a && validL2PTE(d, pg))
     )
 }
 
@@ -231,7 +206,15 @@ predicate validL2PTE(d: PageDb, pte: PageNr)
         && d[pte].entry.DataPage?
 }
 
-predicate closedRefsPageDbEntry(e: PageDbEntryTyped)
+predicate closedRefsPageDbEntry(e: PageDbEntry)
+{
+    e.PageDbEntryFree? ||
+        (e.PageDbEntryTyped?
+        && validPageNr(e.addrspace)
+        && closedRefsPageDbEntryTyped(e.entry))
+}
+
+predicate closedRefsPageDbEntryTyped(e: PageDbEntryTyped)
 {
     (e.Addrspace? && validPageNr(e.l1ptnr) )
     || (e.L1PTable? && closedRefsL1PTable(e))
@@ -253,10 +236,16 @@ predicate closedRefsL2PTable(e: PageDbEntryTyped)
 {
     var l2pt := e.l2pt;
     |l2pt| == NR_L2PTES()
-    // && forall pte :: pte in l2pt ==> (match pte
-    //     case SecureMapping(p, w, e) => validPageNr(p)
-    //     case InsecureMapping(p) => true
-    //     case NoMapping => true)
+    && forall pte :: pte in l2pt ==> closedRefsL2PTE(pte)
+}
+
+predicate closedRefsL2PTE(pte: L2PTE)
+{
+    match pte
+        case SecureMapping(p, w, e) => validPageNr(p)
+        case InsecureMapping(p, w)
+            => 0 <= p < KEVLAR_PHYSMEM_LIMIT() / KEVLAR_PAGE_SIZE()
+        case NoMapping => true
 }
 
 /*
